Definitions for final, initial, undef states.
Also, let typing of states depend on the name of the main function.

smallstep.v
@@ -234,6 +234,13 @@ Inductive cstep `{IntEnv Ti, PtrEnv Ti}
              State k (Stmt (↷ l) (subst Es s)) m
 where "Γ \ δ  ⊢ₛ S1 ⇒ S2" := (@cstep _ _ _ Γ δ S1%S S2%S) : C_scope.
 
+Definition initial_state {Ti} (m : mem Ti)
+  (f : funname) (vs : list (val Ti)) : state Ti := State [] (Call f vs) m.
+Inductive final_state {Ti} (v : val Ti) : state Ti → Prop :=
+  | Return_final m : final_state v (State [] (Return v) m).
+Inductive undef_state {Ti} : state Ti → Prop :=
+  | Undef_undef k Su m : undef_state (State k (Undef Su) m).
+
 (** The reflexive transitive closure. *)
 Notation "Γ \ δ ⊢ₛ S1 ⇒* S2" := (rtc (cstep Γ δ) S1 S2)
   (at level 74, format "Γ \  δ  ⊢ₛ '['  S1  '⇒*' '/'  S2 ']'") : C_scope.
